---
title: "basic q series with R"
author: "Robin K. S. Hankin"
output: html_vignette
bibliography: queueR.bib
vignette: >
  %\VignetteIndexEntry{qbasic}
  %\VignetteEngine{knitr::rmarkdown}
  %\VignetteEncoding{UTF-8}
---


```{r setup, include=FALSE}
knitr::opts_chunk$set(echo = TRUE)
options(rmarkdown.html_vignette.check_title = FALSE)
library("qbasic")
set.seed(1)
```

<p style="text-align: right;">
![](`r system.file("help/figures/qbasic.png", package = "qbasic")`){width=10%}
</p>


To cite the `qbasic` package in publications please use [@rcore2022].
Gasper defines $(a;q)_\infty$ as

$$(a;q)_\infty=\prod_{n=0}^\infty\left(1-aq^n\right)=(1-a)(1-qa)(1-q^2a)\cdots$$

(function `poch()` in the `qbasic` package; Mathematica calls this
`Pochhammer[]`).  Gasper defines the $q$-shifted factorial $(a;q)_n$
as

$$(a;q)_n=(a;q)_\infty/(aq^n;q)_\infty=\underbrace{(1-a)(1-qa)\cdots(1-q^{n-1}a)}_{\mbox{$n$ terms}}$$

The $q$-binomial theorem:

$$\frac{(ax;q)_\infty}{(x;q)_\infty}=\sum_{n=0}^\infty\frac{(a;q)_n}{(q;q)_n}x^n,\qquad\left|x\right|<1$$

The triple product:

$$
(x;q)_\infty\cdot
(qx^{-1};q)_\infty\cdot
(q;q)_\infty=
\sum_{n=-\infty}^\infty(-1)^nq^{n\choose 2}x^n
$$

Gosper gives the slightly different form [dubbed Jacobi's "well-known" triple product identity]:

$$
\left(
zq^\frac{1}{2},q^\frac{1}{2},q;q\right)_\infty
=
\sum_{n=-\infty}^\infty(-1)^nq^{n^2/2}z^n
$$

Gosper defines

$$
\left(a_1,a_2,\ldots,a_m;q\right)_n=
(a_1;q)_n
(a_2;q)_n\cdots
(a_m;q)_n
$$

and 

$$
\left(a_1,a_2,\ldots,a_m;q\right)_\infty=
(a_1;q)_\infty
(a_2;q)_\infty\cdots
(a_m;q)_\infty
$$

Gosper goes on to define

$$
\phi(a,b;c;q,z)=
{}_2\phi_1(a,b;c;q,z)=
{}_2\phi_1\left[
{{a,b}\atop c};q,z\right]
=
\sum_{n=0}^\infty
\frac{
(a;q)_n(b;q)_n}{
(q;q)_n(c;q)_n}z^n
$$


We have the q-gamma function (1.10.1):

$$
\Gamma_q(x)=\frac{(q;q)_\infty}{(q^x;q)_\infty}(1-q)^{1-x}
$$

Gosper shows that $\lim_{q\longrightarrow 1^-}\Gamma_q(x)=\Gamma(x)$,
and goes on (1.10.13) to define the q-beta function:

$$
B_q(x,y)=\frac{\Gamma_q(x)\Gamma_q(y)}{\Gamma_q(x+y)}
$$

and to give a more direct evaluation of it:

$$
B_q(x,y)=(1-q)\sum_{n=0}^\infty\frac{(q^{n+1};q)_\infty}{(q^{n+y};q)_\infty}q^{nx},\qquad
\operatorname{Re}(x),\operatorname{Re}(y)>0
$$




Gosper defines (1.11.3) q-integrals as follows:

$$
\int_0^a f(t)d_qt=a(1-q)\sum_{n=0}^\infty f(aq^n)q^n
$$

with

$$
\int_a^b f(t)d_qt=
\int_0^b f(t)d_qt-\int_0^a f(t)d_qt
$$


If $f$ is continuous on $[0,a]$ we see that $$\lim_{q\longrightarrow
1}\int_0^a f(t)d_qt=\int_0^a f(t)dt$$

1.3.15 1.3.16

$$e_q(z)=\frac{1}{(z;q)_\infty}\qquad |z|<1$$

$$E_q(z)=(-z;q)_\infty$$

We have $e_q(z)E_q(-z)=1$ and

$$
\lim_{q\longrightarrow 1^-}e_q(z(1-q))=\lim_{q\longrightarrow 1^-}E_q(z(1-q))=e^z
$$



## q-Hypergeometric functions

Gasper defines

$$
{}_r\phi_s\left(a_1,\ldots,a_r;b_1,\ldots,b_s;q,z\right)= {}_r\phi_s\left[
{a_1,a_2,\ldots,a_r\atop b_1,\ldots b_s};q,z\right]
$$

$$
=
\sum_{n\geqslant 0}\frac{\left(a_1,\ldots, a_r;q\right)}{\left(q,b_1,\ldots, b_s;q\right)}
\left[(-1)^nq^{n\choose 2}\right] z^n
$$

## References
